DH example finished stateful proofs

examples/dh/DY.Example.DH.Protocol.Stateful.Proof.fst
@@ -14,8 +14,9 @@ open DY.Example.DH.Protocol.Stateful
 /// The (local) state predicate.
 
 val is_dh_shared_key: trace -> principal -> principal -> bytes -> prop
-let is_dh_shared_key tr a b k = exists si sj.
-  is_secret (join (principal_state_label a si) (principal_state_label b sj)) tr k /\ 
+let is_dh_shared_key tr alice bob k = exists si sj.
+  (is_secret (join (principal_state_label alice si) (principal_state_label bob sj)) tr k \/
+  is_secret (join (principal_state_label bob sj) (principal_state_label alice si)) tr k) /\ 
   get_usage k == AeadKey "DH.aead_key"
 
 let dh_session_pred: local_state_predicate dh_session = {
@@ -30,7 +31,6 @@ let dh_session_pred: local_state_predicate dh_session = {
     | ResponderSentMsg2 alice gx gy y -> (
       let bob = prin in
       is_publishable tr gx /\ is_publishable tr gy /\
-      is_knowable_by (principal_state_label bob sess_id) tr y /\
       is_secret (principal_state_label bob sess_id) tr y /\ get_usage y  == DhKey "DH.dh_key" /\
       gy == dh_pk y /\
       event_triggered tr bob (Respond1 alice bob gx gy y)
@@ -40,7 +40,7 @@ let dh_session_pred: local_state_predicate dh_session = {
       is_publishable tr gx /\ is_publishable tr gy /\
       is_knowable_by (principal_state_label alice sess_id) tr k /\
       event_triggered tr alice (Initiate2 alice bob gx gy k) /\
-      (is_corrupt tr (principal_state_label alice sess_id) \/
+      (is_corrupt tr (principal_label alice) \/ is_corrupt tr (principal_label bob) \/
       (exists y. k == dh y gx /\ is_dh_shared_key tr alice bob k /\ 
         event_triggered tr bob (Respond1 alice bob gx gy y)))
     )
@@ -49,8 +49,9 @@ let dh_session_pred: local_state_predicate dh_session = {
       is_publishable tr gx /\ is_publishable tr gy /\
       is_knowable_by (principal_state_label bob sess_id) tr k /\
       event_triggered tr bob (Respond2 alice bob gx gy k) /\
-      (is_corrupt tr (principal_state_label bob sess_id) \/
-      is_dh_shared_key tr alice bob k /\ event_triggered tr alice (Initiate2 alice bob gx gy k))
+      (is_corrupt tr (principal_label alice) \/ is_corrupt tr (principal_label bob) \/
+      (is_dh_shared_key tr alice bob k /\ 
+      event_triggered tr alice (Initiate2 alice bob gx gy k)))
     )
   );
   pred_later = (fun tr1 tr2 prin sess_id st -> ());
@@ -73,11 +74,11 @@ let dh_event_pred: event_predicate dh_event =
       is_publishable tr gx /\ is_publishable tr gy /\
       (exists x sess_id. is_secret (principal_state_label alice sess_id) tr x /\
       gx = dh_pk x) /\
-      (is_corrupt tr (principal_label bob) \/
+      (is_corrupt tr (principal_label alice) \/ is_corrupt tr (principal_label bob) \/
       (exists y. k == dh y gx /\ is_dh_shared_key tr alice bob k /\ event_triggered tr bob (Respond1 alice bob gx gy y)))
     )
     | Respond2 alice bob gx gy k -> (
-      is_corrupt tr (principal_label alice) \/ 
+      is_corrupt tr (principal_label alice) \/ is_corrupt tr (principal_label bob) \/
       (is_dh_shared_key tr alice bob k /\
       event_triggered tr alice (Initiate2 alice bob gx gy k))
     )
@@ -139,3 +140,270 @@ let all_events_has_all_events () =
 
 val full_dh_event_pred_has_dh_invariant: squash (has_event_pred dh_protocol_invs dh_event_pred)
 let full_dh_event_pred_has_dh_invariant = all_events_has_all_events ()
+
+(*** Proofs ****)
+
+val prepare_msg1_proof:
+  tr:trace ->
+  alice:principal -> bob:principal ->
+  Lemma
+  (requires trace_invariant tr)
+  (ensures (
+    let (sess_id, tr_out) = prepare_msg1 alice bob tr in
+    trace_invariant tr_out
+  ))
+let prepare_msg1_proof tr alice bob = ()
+
+val send_msg1_proof:
+  tr:trace ->
+  alice:principal -> bob:principal -> sess_id:nat ->
+  Lemma
+  (requires trace_invariant tr)
+  (ensures (
+    let (msg_id, tr_out) = send_msg1 alice sess_id tr in
+    trace_invariant tr_out
+  ))
+let send_msg1_proof tr alice bob sess_id =
+  match get_state alice sess_id tr with
+  | (Some (InitiatorSentMsg1 bob x), tr) -> (
+    compute_message1_proof tr alice bob x sess_id
+  )
+  | _ -> ()
+
+val prepare_msg2_proof:
+  tr:trace ->
+  alice:principal -> bob:principal -> msg_id:nat ->
+  Lemma
+  (requires trace_invariant tr)
+  (ensures (
+    let (msg_id, tr_out) = prepare_msg2 alice bob msg_id tr in
+    trace_invariant tr_out
+  ))
+let prepare_msg2_proof tr alice bob msg_id =
+  match recv_msg msg_id tr with
+  | (Some msg, tr) -> (
+    decode_message1_proof tr alice bob msg
+  )
+  | (None, tr) -> ()
+
+val send_msg2_proof:
+  tr:trace ->
+  global_sess_id:dh_global_sess_ids -> bob:principal -> sess_id:nat ->
+  Lemma
+  (requires trace_invariant tr)
+  (ensures (
+    let (msg_id, tr_out) = send_msg2 global_sess_id bob sess_id tr in
+    trace_invariant tr_out
+  ))
+let send_msg2_proof tr global_sess_id bob sess_id =
+  match get_state bob sess_id tr with
+  | (Some (ResponderSentMsg2 alice gx gy y), tr) -> (
+    match get_private_key bob global_sess_id.private_keys (Sign "DH.SigningKey") tr with
+    | (Some sk_b, tr) -> (
+      let (n_sig, tr) = mk_rand SigNonce (principal_label bob) 32 tr in
+      compute_message2_proof tr sess_id alice bob {alice; gx} gy y sk_b n_sig
+    )
+    | (None, tr) -> ()
+  )
+  | _ -> ()
+
+#push-options "--z3rlimit 30"
+val prepare_msg3_proof:
+  tr:trace ->
+  global_sess_id:dh_global_sess_ids -> alice:principal -> bob:principal -> msg_id:nat -> sess_id:nat ->
+  Lemma
+  (requires trace_invariant tr)
+  (ensures (
+    let (_, tr_out) = prepare_msg3 global_sess_id alice bob msg_id sess_id tr in
+    trace_invariant tr_out
+  ))
+let prepare_msg3_proof tr global_sess_id alice bob msg_id sess_id =
+  match get_state alice sess_id tr with
+    | (Some (InitiatorSentMsg1 bob x), tr) -> (
+    match recv_msg msg_id tr with
+    | (Some msg_bytes, tr) -> (
+      match get_public_key alice global_sess_id.pki (Verify "DH.SigningKey") bob tr with
+      | (Some pk_b, tr) -> (
+        let gx = dh_pk x in
+        match decode_message2 msg_bytes alice gx pk_b with
+        | Some msg2 -> (
+          decode_message2_proof tr alice bob msg_bytes gx pk_b;
+          let k = dh x msg2.gy in
+          assert(is_publishable tr gx);
+          assert(is_publishable tr msg2.gy);
+          assert(is_knowable_by (principal_state_label alice sess_id) tr k);
+
+          assert((exists x sess_id. is_secret (principal_state_label alice sess_id) tr x /\
+            gx = dh_pk x));
+          assert(get_usage k = AeadKey "DH.aead_key");
+          assert(exists si. is_knowable_by (principal_state_label alice si) tr k);
+
+          introduce (~(is_corrupt tr (principal_label alice) \/ is_corrupt tr (principal_label bob))) ==> (exists y. k == dh y gx /\ is_dh_shared_key tr alice bob k /\ event_triggered tr bob (Respond1 alice bob gx msg2.gy y))
+          with _. (
+            assert(exists y k'. k' == dh y gx /\ msg2.gy == dh_pk y /\ event_triggered tr bob (Respond1 alice bob gx msg2.gy y));
+            eliminate exists y k'. k' == dh y gx /\ event_triggered tr bob (Respond1 alice bob gx msg2.gy y)
+            returns _
+            with _. (
+              assert(event_triggered tr bob (Respond1 alice bob gx msg2.gy y));
+              
+              assert(dh_pk y == msg2.gy);
+              assert(dh_pk x = gx);              
+              dh_shared_secret_lemma x y;
+              assert(dh y gx == dh x msg2.gy);
+              assert(k == k');
+
+              assert(exists si. is_secret (principal_state_label alice si) tr x);
+              assert(exists sj. is_secret (principal_state_label bob sj) tr y);
+              assert(exists si. get_label x == principal_state_label alice si);
+              assert(exists sj. get_label y == principal_state_label bob sj);
+              assert(exists si sj. join (get_label x) (get_label y) == join (principal_state_label alice si) (principal_state_label bob sj));
+
+              normalize_term_spec get_label;
+              reveal_opaque (`%dh) (dh);
+              reveal_opaque (`%dh_pk) (dh_pk);
+              reveal_opaque (`%join) (join);
+              assert(get_label (dh x msg2.gy) == join (get_label x) (get_dh_label msg2.gy) \/
+              get_label (dh x msg2.gy) == join (get_dh_label msg2.gy) (get_label x));
+              
+              assert(exists si sj. is_secret (join (principal_state_label alice si) (principal_state_label bob sj)) tr k \/
+                is_secret (join (principal_state_label bob sj) (principal_state_label alice si)) tr k);
+              ()
+            )
+          )
+        )
+        | None -> ()
+      )
+      | (None, tr) -> ()
+    )
+    | (None, tr) -> ()
+  )
+  | _ -> ()
+#pop-options
+
+val send_msg3_proof:
+  tr:trace ->
+  global_sess_id:dh_global_sess_ids -> alice:principal -> bob:principal -> sess_id:nat ->
+  Lemma
+  (requires trace_invariant tr)
+  (ensures (
+    let (_, tr_out) = send_msg3 global_sess_id alice bob sess_id tr in
+    trace_invariant tr_out
+  ))
+let send_msg3_proof tr global_sess_id alice bob sess_id =
+  match get_state alice sess_id tr with
+  | (Some (InitiatorSendMsg3 bob gx gy k), tr) -> (
+    match get_private_key alice global_sess_id.private_keys (Sign "DH.SigningKey") tr with
+    | (Some sk_a, tr) -> (
+      let (n_sig, tr) = mk_rand SigNonce (principal_label alice) 32 tr in
+
+      (* Debugging code
+      assert(event_triggered tr alice (Initiate2 alice bob gx gy k));
+      assert(exists x. gx == dh_pk x); *)
+
+      compute_message3_proof tr sess_id alice bob gx gy sk_a n_sig;
+      ()
+    )
+    | (None, tr) -> ()
+  )
+  | _ -> ()
+
+val event_respond1_injective:
+  tr:trace ->
+  alice:principal -> bob:principal ->
+  gx:bytes -> gy:bytes -> y:bytes -> y':bytes ->
+  Lemma
+  (requires 
+    trace_invariant tr /\
+    event_triggered tr bob (Respond1 alice bob gx gy y) /\
+    event_triggered tr bob (Respond1 alice bob gx gy y')
+  )
+  (ensures
+    y == y'
+  )
+let event_respond1_injective tr alice bob gx gy y y' =  
+  reveal_opaque (`%dh_pk) (dh_pk);
+  assert(gy == dh_pk y);
+  assert(gy == dh_pk y');
+  assert(y == y');
+  ()
+
+#push-options "--z3rlimit 40"
+val verify_msg3_proof:
+  tr:trace ->
+  global_sess_id:dh_global_sess_ids -> alice:principal -> bob:principal -> msg_id:nat -> sess_id:nat ->
+  Lemma
+  (requires trace_invariant tr)
+  (ensures (
+    let (_, tr_out) = verify_msg3 global_sess_id alice bob msg_id sess_id tr in
+    trace_invariant tr_out
+  ))
+let verify_msg3_proof tr global_sess_id alice bob msg_id sess_id =
+  match get_state bob sess_id tr with
+  | (Some (ResponderSentMsg2 alice gx gy y), tr) -> (
+    match recv_msg msg_id tr with
+    | (Some msg_bytes, tr) -> (
+      match get_public_key bob global_sess_id.pki (Verify "DH.SigningKey") alice tr with
+      | (Some pk_a, tr) -> (
+          decode_message3_proof tr alice bob gx gy msg_bytes pk_a;
+          
+          match decode_message3 msg_bytes bob gx gy pk_a with
+          | Some msg3 -> (
+            
+            let k = dh y gx in
+
+            assert(event_triggered tr bob (Respond1 alice bob gx gy y));
+            // The decode_message3_proof gives us that there exists a k' such that 
+            // the event Initiate2 has been triggered or alice is corrupt.
+            // On a high level we need to show now that this event was triggered
+            // for our concrete k.
+            assert(exists k'. event_triggered tr alice (Initiate2 alice bob gx gy k') \/ is_corrupt tr (principal_label alice));
+
+            // Proof strategy: We want to work without the corruption case
+            // so we introduce this implication. 
+            introduce (~((principal_label alice) `can_flow tr` public \/ (principal_label bob) `can_flow tr` public)) ==> event_triggered tr alice (Initiate2 alice bob gx gy k) with _. (
+              // We can now assert that there exists a k' such that the event Initiate2 has been triggered
+              // without the corruption case.
+              assert(exists k'. event_triggered tr alice (Initiate2 alice bob gx gy k'));
+              // We now introduce k' to concretely reason about it.
+              eliminate exists k'. event_triggered tr alice (Initiate2 alice bob gx gy k')
+              returns _
+              with _. (
+                // From the Initiate2 event we know that there exists a Respond1 event with 
+                // gx, gy and some y'. To show that k equals k' it is enough to show that
+                // y' equals y since k = dh y gx.       
+                assert(exists y'. k' == dh y' gx /\ event_triggered tr bob (Respond1 alice bob gx gy y'));
+                
+                // To concretely reason about y' we introduce it via an elimination.
+                eliminate exists y'. gy == dh_pk y' /\ k' == dh y' gx /\ event_triggered tr bob (Respond1 alice bob gx gy y')
+                returns _
+                with _. (
+                  // The event_respond1_injective lemma gives us that the
+                  // event triggered with y and y' is the same
+                  event_respond1_injective tr alice bob gx gy y y';
+                  // With the lemma above F* can automatically deduce that
+                  // k and k' must be equal.
+                  assert(k == k');
+                  // This gives us that the event Initiate2 has been triggered
+                  // for our concrete k.
+                  assert(event_triggered tr alice (Initiate2 alice bob gx gy k));
+                  assert(event_triggered tr alice (Initiate2 alice bob gx gy k'));
+                  ()
+                )
+              )
+            );
+ 
+            assert(is_corrupt tr (principal_label alice) \/ is_corrupt tr (principal_label bob) \/ 
+              (exists si sj. is_secret (join (principal_state_label alice si) (principal_state_label bob sj)) tr k \/
+                is_secret (join (principal_state_label bob sj) (principal_state_label alice si)) tr k));
+            assert(get_usage k == AeadKey "DH.aead_key");
+            assert(is_corrupt tr (principal_label alice) \/ is_corrupt tr (principal_label bob) \/
+              (is_dh_shared_key tr alice bob k /\ event_triggered tr alice (Initiate2 alice bob gx gy k)));
+            ()
+          )
+          | None -> ()
+        )
+        | (None, tr) -> ()
+      )
+      | (None, tr) -> ()
+    )
+  | (_, tr) -> ()
